\documentclass[a4paper,11pt]{scrartcl}
\usepackage[utf8]{inputenc}
\usepackage[english]{babel}

\usepackage[headsepline]{scrlayer-scrpage}
\ohead{Bernd Schwarzenbacher}
\ihead{HW1}

\usepackage{amsmath}
\usepackage{amssymb}
\usepackage{commath}
\usepackage[retainorgcmds]{IEEEtrantools}

\usepackage{amsthm}

\newcommand*{\dt}{\dif{}t}
\newcommand*{\dW}{\dif{}W_t}
\newcommand*{\Sm}[1]{\sum_{n=0}^{N-1}{#1}}
\newcommand*{\Smm}[1]{\sum_{m=0}^{N-1}{#1}}
\newcommand*{\D}{\Delta}
\newcommand*{\E}{\mathbb{E}}
\newcommand*{\EV}[1]{\E\left[{#1}\right]}

\begin{document}
We show that: \[\int_0^T{W_t \dW} = \frac{W(T)^2}{2} - \frac{T}{2}\]
The Euler discretization of the integral is $\Sm{W(t_{n})\D W_n}$.
To get the first term of the right hand side we can add the square increments:
\begin{IEEEeqnarray*}{rCl}
  2 \Sm{W(t_{n})\D W} + \Sm{(\D W_n)^2} & = & 
  2 \Sm{W(t_{n})(W(t_{n+1}) - W(t_{n}))} \\
  & &
  + \Sm{(W(t_{n+1}) - W(t_{n}))(W(t_{n+1}) - W(t_{n}))} \\
  & = & \Sm{(W(t_{n+1}) + W(t_{n}))(W(t_{n+1}) - W(t_{n}))} \\
  & = & \Sm{W(t_{n+1})^2 - W(t_n)^2} = W(T)^2 - W(0)^2 = W(T)^2 \\
\end{IEEEeqnarray*}
To get the second term, observe that the increments of a Wiener process are normaly distributed with
variance $\EV{(\D W_n)^2} = \D t_n$ and
the kurtosis for the normal distribution is $3$ so $\EV{(\D W_n)^4} = 3 (\D
t_n)^2$
This and the independence of the increments together with $\EV{(\D W_n)^2 - \D t_n} = 0$
gets rid of the cross terms in the following:
\[
  \EV{ \left( \Sm{(\D W_n)^2} - T \right)^2 } =
  \EV{ \left( \Sm{(\D W_n)^2} - \Sm{\D t_n} \right)^2 } \]
\[ =
  \EV{\Sm{(\D W_n)^4 - 2 (\D W_n)^2 \D t_n + (\D t_n)^2}} \]
\[  = \Sm{3 (\D t_n)^2 - 2 (\D t_n)^2 + (\D t_n)^2}  = 2 \Sm{(\D t_n)^2} \leq 2
  T \max_n{\D t_n} \rightarrow 0\]
Which all together gives:
\[ \Sm{W(t_n) \D W_n} \overset{\bold{L}^2}{\longrightarrow} \frac{W(T)^2}{2} - \frac{T}{2}\]
As the $\bold{L}^2$-limit of the forward Euler discretization is the definition of the
It\^{o} integral we arrived at the desired equality.

\pagebreak
We show that:
\[ \EV{\int_0^T f(t, \cdot) \dW \int_0^T g(t, \cdot) \dW} = \int_0^T
  \EV{f(t,\cdot) g(t, \cdot)} \dt \]
We start by showing, that the Euler discretizations are equal:
\begin{IEEEeqnarray*}{rR}
\EV{\Sm{f(t_n, \cdot) \D W(t_n) \Sm{g(t_n, \cdot) \D W(t_n)}}} & = \\
\Sm{\Smm{\EV{f(t_m, \cdot) \D W(t_m) g(t_n, \cdot) \D W(t_n)}}} & = \\
2 \sum_{n < m}^{N-1}{\EV{f(t_m, \cdot) \D W(t_m) g(t_n, \cdot) \D W(t_n)}} +
\sum_{n=0}^{N-1}{\EV{f(t_n, \cdot) g(t_n, \cdot) (\D W(t_n))^2}} \\
\end{IEEEeqnarray*}
We now use, that $f$ and $g$ are adapted and the independence of the increments:
\[
2 \sum_{n < m}^{N-1}{\EV{\D W(t_m)}\EV{f(t_m, \cdot) g(t_n, \cdot) \D W(t_n)}} +
\sum_{n=0}^{N-1}{\EV{(\D W(t_n))^2}\EV{f(t_n, \cdot) g(t_n, \cdot)}}
\]
For the first term we use $\EV{\D W(t_m)} = 0$ and for the second term
$\EV{(\D W(t_n))^2} = \D t$ to get
\[ \sum_{n=0}^{N-1}{\D t_n \EV{f(t_n, \cdot) g(t_n, \cdot)}} \]
Now we can add the two equal Euler discretizations as $0$:
\begin{IEEEeqnarray*}{rR}
  \left|
    \EV{\int_0^T f(t, \cdot) \dW \int_0^T g(t, \cdot) \dW}
    - \int_0^T \EV{f(t,\cdot) g(t, \cdot)} \dt
  \right| & = \\
  \left|
    \EV{\int_0^T f(t, \cdot) \dW \int_0^T g(t, \cdot) \dW}
    - \EV{\Sm{f(t_n, \cdot) \D W(t_n) \Sm{g(t_n, \cdot) \D W(t_n)}}}
  \right. & \\
  \left.
    + \sum_{n=0}^{N-1}{\EV{f(t_n, \cdot) g(t_n, \cdot)} \D t_n}
    - \int_0^T \EV{f(t,\cdot) g(t, \cdot)} \dt
  \right| & \leq \\
  \sqrt{ \EV{ \left(
        \int_0^T f(t, \cdot) \dW \int_0^T g(t, \cdot) \dW
        - \Sm{f(t_n, \cdot) \D W(t_n) \Sm{g(t_n, \cdot) \D W(t_n)}}
  \right)^2 } } & \\
  + \left|
    \sum_{n=0}^{N-1}{\EV{f(t_n, \cdot) g(t_n, \cdot)} \D t_n}
    - \int_0^T \EV{f(t,\cdot) g(t, \cdot)} \dt
  \right| & \rightarrow 0
\end{IEEEeqnarray*}
The first term converges to zero by definition of the It\^{o} integral and the
second term by definition of the Riemann integral.

\end{document}